TypeInference.v
@@ -9,7 +9,7 @@ Section ErrorReporting.
 
   Inductive error_message :=
   | UnboundVariable (var: var_t)
-  | TypeMismatch {sig tau} (e: expr var_t R Sigma sig tau) (expected: type).
+  | TypeMismatch {sig tau} (e: action var_t R Sigma sig tau) (expected: type).
 
   Record error :=
     { epos: pos_t;
@@ -27,14 +27,12 @@ Section TypeInference.
   Context (Sigma: fn_t -> ExternalSignature).
   Context (uSigma: forall (fn: ufn_t) (tau1 tau2: type), fn_t).
 
-  Notation uexpr := (uexpr pos_t var_t reg_t ufn_t).
-  Notation urule := (urule pos_t var_t reg_t ufn_t).
+  Notation uaction := (uaction pos_t var_t reg_t ufn_t).
   Notation uscheduler := (uscheduler pos_t name_t).
 
   Open Scope bool_scope.
 
-  Notation expr := (expr var_t R Sigma).
-  Notation rule := (rule var_t R Sigma).
+  Notation action := (action var_t R Sigma).
   Notation scheduler := (scheduler name_t).
   Notation schedule := (schedule name_t var_t R Sigma).
   Notation error := (error pos_t var_t R Sigma).
@@ -70,10 +68,10 @@ Section TypeInference.
      end)
       (at level 200).
 
-  Section Expr.
-    Definition cast_expr (pos: pos_t)
-               sig {tau1} tau2 (e: expr sig tau1)
-      : result (expr sig tau2).
+  Section Action.
+    Definition cast_action (pos: pos_t)
+               sig {tau1} tau2 (e: action sig tau1)
+      : result (action sig tau2).
     Proof.
       destruct (eq_dec tau1 tau2); subst.
       - exact (WellTyped e).
@@ -83,61 +81,54 @@ Section TypeInference.
 
     Notation EX Px := (existT _ _ Px).
 
-    Fixpoint expos pos (e: uexpr) :=
+    Fixpoint actpos pos (e: uaction) :=
       match e with
-      | UEPos p _ => p
+      | UAPos p _ => p
       | _ => pos
       end.
 
     Definition unbound_variable pos var : error :=
       {| epos := pos; emsg := UnboundVariable var |}.
 
-    Fixpoint type_expr (pos: pos_t) (sig: tsig var_t) (e: uexpr)
-      : result ({ tau: type & expr sig tau }) :=
+    Fixpoint type_action (pos: pos_t) (sig: tsig var_t) (e: uaction)
+      : result ({ tau: type & action sig tau }) :=
       match e with
+      | UFail n => WellTyped (EX (Fail (bits_t n)))
       | UVar var =>
         let/res ktau_m := opt_result (assoc var sig) (unbound_variable pos var) in
         WellTyped (EX (Var ``ktau_m))
       | UConst cst => WellTyped (EX (Const cst))
-      | URead port idx => WellTyped (EX (Read port idx))
-      | UCall ufn arg1 arg2 =>
-        let/res arg1' := type_expr pos sig arg1 in
-        let/res arg2' := type_expr pos sig arg2 in
-        let fn := uSigma ufn `arg1' `arg2' in
-        let/res arg1' := cast_expr (expos pos arg1) sig (Sigma fn).(arg1Type) (``arg1') in
-        let/res arg2' := cast_expr (expos pos arg2) sig (Sigma fn).(arg2Type) (``arg2') in
-        WellTyped (EX (Call fn arg1' arg2'))
-      | UEPos pos e => type_expr pos sig e
-      end.
-  End Expr.
-
-  Section Rule.
-    Fixpoint type_rule (pos: pos_t) (sig: tsig var_t)
-             (r: urule) : result (rule sig) :=
-      match r with
-      | USkip => WellTyped Skip
-      | UFail => WellTyped Fail
       | USeq r1 r2 =>
-        let/res r1 := type_rule pos sig r1 in
-        let/res r2 := type_rule pos sig r2 in
-        WellTyped (Seq r1 r2)
+        let/res r1' := type_action pos sig r1 in
+        let/res r1' := cast_action (actpos pos r1) sig (bits_t 0) (``r1') in
+        let/res r2' := type_action pos sig r2 in
+        WellTyped (EX (Seq r1' ``r2'))
       | UBind v ex body =>
-        let/res ex := type_expr pos sig ex in
-        let/res body := type_rule pos ((v, `ex) :: sig) body in
-        WellTyped (Bind v ``ex body)
+        let/res ex := type_action pos sig ex in
+        let/res body := type_action pos ((v, `ex) :: sig) body in
+        WellTyped (EX (Bind v ``ex ``body))
       | UIf cond tbranch fbranch =>
-        let/res cond' := type_expr pos sig cond in
-        let/res tbranch := type_rule pos sig tbranch in
-        let/res fbranch := type_rule pos sig fbranch in
-        let/res cond' := cast_expr (expos pos cond) sig (bits_t 1) (``cond') in
-        WellTyped (If cond' tbranch fbranch)
+        let/res cond' := type_action pos sig cond in
+        let/res cond' := cast_action (actpos pos cond) sig (bits_t 1) (``cond') in
+        let/res tbranch' := type_action pos sig tbranch in
+        let/res fbranch' := type_action pos sig fbranch in
+        let/res fbranch' := cast_action (actpos pos fbranch) sig (`tbranch') (``fbranch') in
+        WellTyped (EX (If cond' ``tbranch' fbranch'))
+      | URead port idx => WellTyped (EX (Read port idx))
       | UWrite port idx value =>
-        let/res value' := type_expr pos sig value in
-        let/res value' := cast_expr (expos pos value) sig (R idx) (``value') in
-        WellTyped (Write port idx value')
-      | URPos pos r => type_rule pos sig r
+        let/res value' := type_action pos sig value in
+        let/res value' := cast_action (actpos pos value) sig (R idx) (``value') in
+        WellTyped (EX (Write port idx value'))
+      | UCall ufn arg1 arg2 =>
+        let/res arg1' := type_action pos sig arg1 in
+        let/res arg2' := type_action pos sig arg2 in
+        let fn := uSigma ufn `arg1' `arg2' in
+        let/res arg1' := cast_action (actpos pos arg1) sig (Sigma fn).(arg1Type) (``arg1') in
+        let/res arg2' := cast_action (actpos pos arg2) sig (Sigma fn).(arg2Type) (``arg2') in
+        WellTyped (EX (Call fn arg1' arg2'))
+      | UAPos pos e => type_action pos sig e
       end.
-  End Rule.
+  End Action.
 
   Section Scheduler.
     Fixpoint type_scheduler
@@ -165,24 +156,36 @@ Arguments IllTyped {_ _ _ _ R Sigma A}.
 
 (* Coq bug: the name must_typecheck is not resolved at notation definition time *)
 
-Notation _must_typecheck R Sigma tcres :=
-  ltac:(let tcres := (eval hnf in tcres) in
-        let tcterm := (eval cbn in (must_typecheck R Sigma tcres)) in
-        exact tcterm) (only parsing).
+Ltac __must_typecheck_cbn R Sigma tcres :=
+  let tcres := (eval hnf in tcres) in
+  let tcterm := (eval cbn in (must_typecheck R Sigma tcres)) in
+  exact tcterm.
 
-Notation tc_rule R Sigma uSigma rule :=
-  (ltac:(let typed := constr:(type_rule R Sigma uSigma tt List.nil rule) in
-         exact (_must_typecheck R%function Sigma%function typed)))
+(* This version is much faster, but it unfolds everything *)
+Ltac __must_typecheck_cbv R Sigma tcres :=
+  let tcterm := (eval cbv in (must_typecheck R Sigma tcres)) in
+  exact tcterm.
+
+Ltac __must_typecheck R Sigma tcres :=
+  __must_typecheck_cbv R Sigma tcres.
+
+Notation _must_typecheck R Sigma tcres :=
+  ltac:(__must_typecheck R Sigma tcres) (only parsing).
+
+Notation tc_action R Sigma uSigma action :=
+  (ltac:(let typed := constr:(type_action R Sigma uSigma tt List.nil action) in
+         let typed := eval cbn in (projT2 (_must_typecheck R%function Sigma%function typed)) in
+         exact typed))
     (only parsing).
 
-Notation tc_rules R Sigma uSigma rules :=
-  (ltac:(match type of rules with
+Notation tc_rules R Sigma uSigma actions :=
+  (ltac:(match type of actions with
          | (?name_t -> _) =>
            let res := constr:(fun r: name_t =>
                                ltac:(destruct r eqn:? ;
                                        lazymatch goal with
                                        | [ H: _ = ?rr |- _ ] =>
-                                         exact (tc_rule R Sigma uSigma (rules rr))
+                                         exact (tc_action R Sigma uSigma (actions rr))
                                        end)) in
            let res := (eval cbn in res) in
            exact res
@@ -210,14 +213,14 @@ Notation tc_scheduler uscheduler :=
 (*                   H': getenv ?env ?k = Some ?v |- _ ] => *)
 (*              pose_once (and_fst H k v) H' *)
 (*            | [ H: forall Gamma gamma tau, _ -> _ = Some _ -> _, *)
-(*                  H': type_expr ?Gamma ?r = Some ?tau |- _ ] => *)
+(*                  H': type_action ?Gamma ?r = Some ?tau |- _ ] => *)
 (*              specialize (H Gamma _ tau ltac:(eauto with types) H') *)
 (*            | [ H: MaxType ?R ?Sigma ?Gamma ?r ?tau |- _ ] => *)
 (*              pose_once (MaxType_HasType R Sigma Gamma r tau) H *)
 (*            | _ => solve [econstructor] || econstructor; solve [eauto 5 with types] *)
 (*            end. *)
 
-(*    Lemma type_expr_correct_call: *)
+(*    Lemma type_action_correct_call: *)
 (*     forall sigma v, *)
 (*       env_related id v R -> *)
 (*       env_related id sigma Sigma -> *)
@@ -228,11 +231,11 @@ Notation tc_scheduler uscheduler :=
 (*          List.Forall *)
 (*            (fun r : rule var_t fn_t => *)
 (*               forall Gamma gamma tau, *)
-(*                 env_related id gamma Gamma -> type_expr Gamma r = Some tau -> MaxType v sigma gamma r tau) args -> *)
+(*                 env_related id gamma Gamma -> type_action Gamma r = Some tau -> MaxType v sigma gamma r tau) args -> *)
 (*          fold_right2 *)
 (*            (fun arg argSize acc => *)
 (*               acc && *)
-(*                   match type_expr Gamma arg with *)
+(*                   match type_action Gamma arg with *)
 (*                   | Some tau => if type_le_dec (bits_t argSize) tau then true else false *)
 (*                   | None => false *)
 (*                   end) true args argSizes = true -> *)
@@ -243,26 +246,26 @@ Notation tc_scheduler uscheduler :=
 (*      induction args; destruct argSizes; cbn in *; *)
 (*        inversion 1; intros ? ? ?; inversion 1; subst; intros Heq. *)
 (*      - eauto. *)
-(*      - destruct type_expr eqn:?; *)
+(*      - destruct type_action eqn:?; *)
 (*          apply andb_prop in Heq; repeat cleanup_step. *)
 (*        destruct type_le_dec; try discriminate. *)
 (*        eauto using MaxType_HasType. *)
 (*    Qed. *)
 
-(*   Lemma type_expr_correct : *)
+(*   Lemma type_action_correct : *)
 (*     forall sigma v, *)
 (*       env_related id v R -> *)
 (*       env_related id sigma Sigma -> *)
 (*       forall (r: rule var_t fn_t) (Gamma: GammaEnv.(env_t)) gamma (tau: type), *)
 (*         env_related id gamma Gamma -> *)
-(*         type_expr Gamma r = Some tau -> *)
+(*         type_action Gamma r = Some tau -> *)
 (*         MaxType v sigma gamma r tau. *)
 (*   Proof. *)
 (*     induction r using rule_ind'; cbn; intros; t. *)
 
 (*     econstructor; eauto. *)
 (*     eapply fold_right2_forall2; *)
-(*       eauto using type_expr_correct_call. *)
+(*       eauto using type_action_correct_call. *)
 (*   Qed. *)
 
 (*   Lemma forall2_cons_inv {A B} (P: A -> B -> Prop) : *)
@@ -288,22 +291,22 @@ Notation tc_scheduler uscheduler :=
 (*       apply HasType_MaxType in H; destruct H as (? & ? & ?) *)
 (*     | [ H: ?x = Some _ |- opt_bind ?x _ = _ ] => *)
 (*       rewrite H; cbn *)
-(*     | [ H: (forall _ _ , _ -> forall _, _ -> type_expr _ ?r  = Some _)  |- *)
-(*         opt_bind (type_expr _ ?r) _ = Some _ ] => *)
+(*     | [ H: (forall _ _ , _ -> forall _, _ -> type_action _ ?r  = Some _)  |- *)
+(*         opt_bind (type_action _ ?r) _ = Some _ ] => *)
 (*       erewrite H by eauto with types; cbn *)
 (*     | [ H: type_le ?x ?y |- context[type_le_dec ?x ?y] ] => *)
 (*       destruct type_le_dec; try tauto *)
 (*     | _ => cleanup_step *)
 (*     end. *)
 
-(*   Lemma type_expr_complete_call: *)
+(*   Lemma type_action_complete_call: *)
 (*     forall (sigma : fenv fn_t ExternalSignature) (v : fenv nat nat) (args : list (rule var_t fn_t)) argSizes, *)
 (*       length args = length argSizes -> *)
 (*       List.Forall *)
 (*         (fun r : rule var_t fn_t => *)
 (*            forall (gamma : fenv var_t type) (tau : type), *)
 (*              MaxType v sigma gamma r tau -> *)
-(*              forall Gamma : env_t GammaEnv, fenv_related gamma Gamma -> type_expr Gamma r = Some tau) args -> *)
+(*              forall Gamma : env_t GammaEnv, fenv_related gamma Gamma -> type_action Gamma r = Some tau) args -> *)
 (*       forall (gamma : fenv var_t type) (Gamma : env_t GammaEnv), *)
 (*         forall2 (fun (arg : rule var_t fn_t) (argSize : nat) => HasType v sigma gamma arg (bits_t argSize)) args argSizes -> *)
 (*         fenv_related gamma Gamma -> *)
@@ -311,7 +314,7 @@ Notation tc_scheduler uscheduler :=
 (*           fold_right2 *)
 (*             (fun (arg : rule var_t fn_t) (argSize : nat) (acc : bool) => *)
 (*              acc && *)
-(*              match type_expr Gamma arg with *)
+(*              match type_action Gamma arg with *)
 (*              | Some tau0 => if type_le_dec (bits_t argSize) tau0 then true else false *)
 (*              | None => false *)
 (*              end) b args argSizes = b. *)
@@ -329,7 +332,7 @@ Notation tc_scheduler uscheduler :=
 (*       eauto. *)
 (*   Qed. *)
 
-(*   Lemma type_expr_complete : *)
+(*   Lemma type_action_complete : *)
 (*     forall sigma v, *)
 (*       fenv_related v R -> *)
 (*       fenv_related sigma Sigma -> *)
@@ -337,31 +340,31 @@ Notation tc_scheduler uscheduler :=
 (*         MaxType v sigma gamma r tau -> *)
 (*         forall (Gamma: GammaEnv.(env_t)), *)
 (*         fenv_related gamma Gamma -> *)
-(*         type_expr Gamma r = Some tau. *)
+(*         type_action Gamma r = Some tau. *)
 (*   Proof. *)
 (*     induction r using rule_ind'; cbn; inversion 1; *)
 (*       repeat tcomplete_step; eauto using f_equal with types. *)
 
 (*     - destruct PeanoNat.Nat.eq_dec; try tauto. *)
-(*       erewrite type_expr_complete_call; eauto. *)
+(*       erewrite type_action_complete_call; eauto. *)
 (*   Qed. *)
 
 (*   Theorem TypeInference : *)
 (*     forall Gamma (r: rule var_t fn_t), *)
-(*       match type_expr Gamma r with *)
+(*       match type_action Gamma r with *)
 (*       | Some tau => HasType (tenv_of_env id R) (tenv_of_env id Sigma) (tenv_of_env id Gamma) r tau *)
 (*       | None => forall tau, not (HasType (tenv_of_env id R) (tenv_of_env id Sigma) (tenv_of_env id Gamma) r tau) *)
 (*       end. *)
 (*   Proof. *)
-(*     intros; destruct type_expr eqn:?. *)
+(*     intros; destruct type_action eqn:?. *)
 (*     - eapply MaxType_HasType. *)
-(*       + eapply type_expr_correct; *)
+(*       + eapply type_action_correct; *)
 (*           try eapply tenv_of_env_related; eauto. *)
 (*       + eauto with types. *)
 (*     - intros tau Habs. *)
 (*       eapply HasType_MaxType in Habs. *)
 (*       destruct Habs as (? & Habs & Hle). *)
-(*       eapply type_expr_complete in Habs; *)
+(*       eapply type_action_complete in Habs; *)
 (*         try eapply tenv_of_env_frelated. *)
 (*       congruence. *)
 (*   Qed. *)
